Updates.

FOL/Sub/All/Rec/SubAllRecChangeReplaceFree.lean
@@ -1,4 +1,13 @@
+import FOL.Formula
+import FOL.Binders
+import FOL.FunctionUpdateIte
+
 import Mathlib.Data.String.Lemmas
+
+
+namespace FOL
+
+open Formula
 
 
 def List.str_max_len :
@@ -31,7 +40,8 @@ lemma list_str_max_len_mem
 def variant
   (s : String)
   (c : Char)
-  (l : List String) :=
+  (l : List String) :
+  String :=
   if h : s ∈ l
   then
   have : List.str_max_len l + 1 - (String.length s + String.length (Char.toString c)) < List.str_max_len l + 1 - String.length s :=
@@ -76,3 +86,160 @@ lemma variant_spec
     simp [if_neg h]
     exact h
   termination_by variant_spec s _ l => List.str_max_len l + 1 - s.length
+
+
+def Finset.str_max_len :
+  Finset String → ℕ :=
+  Finset.fold (fun x x_1 => max x x_1) 0 String.length
+
+lemma finset_str_max_len_mem
+  (s : String)
+  (l : Finset String)
+  (h1 : s ∈ l) :
+  s.length <= Finset.str_max_len l :=
+  by
+  induction l using Finset.induction_on
+  case empty =>
+    simp at h1
+  case insert hd tl a1 ih =>
+    simp at h1
+    cases h1
+    case inl c1 =>
+      subst c1
+      unfold Finset.str_max_len
+      simp
+    case inr c1 =>
+      unfold Finset.str_max_len at ih
+      unfold Finset.str_max_len
+      simp
+      right
+      exact ih c1
+
+def FinsetVariant
+  (s : String)
+  (c : Char)
+  (l : Finset String) :
+  String :=
+  if h : s ∈ l
+  then
+  have : Finset.str_max_len l + 1 - (String.length s + String.length (Char.toString c)) < Finset.str_max_len l + 1 - String.length s :=
+    by
+    have s1 : (Char.toString c).length = 1
+    rfl
+
+    simp only [s1]
+    simp
+    obtain s2 := finset_str_max_len_mem s l h
+    simp only [tsub_lt_tsub_iff_right s2]
+    simp
+  FinsetVariant (s ++ c.toString) c l
+  else s
+  termination_by FinsetVariant s _ l => Finset.str_max_len l + 1 - s.length
+
+
+lemma variant_spec'
+  (s : String)
+  (c : Char)
+  (l : Finset String) :
+  ¬ FinsetVariant s c l ∈ l :=
+  if h : s ∈ l
+  then
+  have : Finset.str_max_len l + 1 - (String.length s + String.length (Char.toString c)) < Finset.str_max_len l + 1 - String.length s :=
+    by
+    have s1 : (Char.toString c).length = 1
+    rfl
+
+    simp only [s1]
+    simp
+    obtain s2 := finset_str_max_len_mem s l h
+    simp only [tsub_lt_tsub_iff_right s2]
+    simp
+  by
+    unfold FinsetVariant
+    simp
+    simp only [if_pos h]
+    apply variant_spec'
+  else by
+    unfold FinsetVariant
+    simp
+    simp [if_neg h]
+    exact h
+  termination_by variant_spec' s _ l => Finset.str_max_len l + 1 - s.length
+
+
+def Finset.var_name_max_len :
+  Finset VarName → ℕ :=
+  Finset.fold (fun x x_1 => max x x_1) 0 (String.length ∘ VarName.toString)
+
+lemma finset_var_name_max_len_mem
+  (s : VarName)
+  (l : Finset VarName)
+  (h1 : s ∈ l) :
+  s.length <= Finset.var_name_max_len l :=
+  by
+  induction l using Finset.induction_on
+  case empty =>
+    simp at h1
+  case insert hd tl a1 ih =>
+    simp at h1
+    cases h1
+    case inl c1 =>
+      subst c1
+      unfold Finset.var_name_max_len
+      simp
+    case inr c1 =>
+      unfold Finset.var_name_max_len at ih
+      unfold Finset.var_name_max_len
+      simp
+      right
+      exact ih c1
+
+def FinsetVarNameVariant
+  (s : VarName)
+  (c : Char)
+  (l : Finset VarName) :
+  VarName :=
+  if h : s ∈ l
+  then
+  have : Finset.var_name_max_len l + 1 - (s.length + String.length (Char.toString c)) < Finset.var_name_max_len l + 1 - s.length :=
+    by
+    have s1 : (Char.toString c).length = 1
+    rfl
+
+    simp only [s1]
+    simp
+    obtain s2 := finset_var_name_max_len_mem s l h
+    simp only [tsub_lt_tsub_iff_right s2]
+    simp
+  FinsetVarNameVariant (VarName.mk (s.toString ++ c.toString)) c l
+  else s
+  termination_by FinsetVarNameVariant s _ l => Finset.var_name_max_len l + 1 - s.length
+
+
+def subVariant
+  (σ : VarName → VarName)
+  (c : Char) :
+  Formula → Formula
+| pred_const_ X xs => pred_const_ X (xs.map σ)
+| pred_var_ X xs => pred_var_ X (xs.map σ)
+| eq_ x y => eq_ (σ x) (σ y)
+| true_ => true_
+| false_ => false_
+| not_ phi => not_ (subVariant σ c phi)
+| imp_ phi psi => imp_ (subVariant σ c phi) (subVariant σ c psi)
+| and_ phi psi => and_ (subVariant σ c phi) (subVariant σ c psi)
+| or_ phi psi => or_ (subVariant σ c phi) (subVariant σ c psi)
+| iff_ phi psi => iff_ (subVariant σ c phi) (subVariant σ c psi)
+| forall_ x phi =>
+  let x' : VarName :=
+    if ∃ (y : VarName), y ∈ phi.freeVarSet \ {x} ∧ x = σ y
+    then FinsetVarNameVariant x c ((subVariant (Function.updateIte σ x x) c phi).freeVarSet)
+    else x
+  forall_ x' (subVariant (Function.updateIte σ x x') c phi)
+| exists_ x phi =>
+  let x' : VarName :=
+    if ∃ (y : VarName), y ∈ phi.freeVarSet \ {x} ∧ x = σ y
+    then FinsetVarNameVariant x c ((subVariant (Function.updateIte σ x x) c phi).freeVarSet)
+    else x
+  exists_ x' (subVariant (Function.updateIte σ x x') c phi)
+| def_ X xs => def_ X (xs.map σ)
